intermediate commit to go back to

src/PlutusIR/Semantics/Static/normaliser_STLC/gu_naive/SN_STLC_named_naive.v
@@ -14,12 +14,21 @@ Set Implicit Arguments.
 Unset Strict Implicit.
 Unset Printing Implicit Defensive.
 From PlutusCert Require Import STLC_named STLC_named_typing ARS.
-From PlutusCert Require Import alpha alpha_rename rename util alpha_ctx_sub freshness alpha_freshness alpha_step step alpha_sub.
+From PlutusCert Require Import alpha alpha_rename rename util alpha_ctx_sub freshness alpha_freshness.
 
-(* TODO: Used to be Prop. Ask Jacco*)
+Fixpoint sub (X : string) (U T : term) : term :=
+  match T with
+  | tmvar Y =>
+    if X =? Y then U else tmvar Y
+  | tmlam Y K1 T' =>
+    tmlam Y K1 (sub X U T')
+  | tmapp T1 T2 =>
+    tmapp (sub X U T1) (sub X U T2)
+  end.
+
 Inductive step_naive : term -> term -> Set :=
 | step_beta (x : string) (A : type) (s t : term) :
-    step_naive (tmapp (tmlam x A s) t) ( substituteT x t s)
+    step_naive (tmapp (tmlam x A s) t) ( sub x t s)
 | step_appL s1 s2 t :
     step_naive s1 s2 -> step_naive (tmapp s1 t) (tmapp s2 t)
 | step_appR s t1 t2 :
@@ -27,7 +36,54 @@ Inductive step_naive : term -> term -> Set :=
 | step_abs x A s1 s2 :
     step_naive s1 s2 -> step_naive (tmlam x A s1) (tmlam x A s2).
 
-Definition to_unique_binders (s : term) := s.
+Fixpoint subs (sigma : list (string * term)) (T : term) : term :=
+  match sigma with
+  | nil => T
+  | cons (x, t) sigma' => sub x t (subs sigma' T) (* or the other way around?*)
+  end.
+
+(* Define the rewrite rules *)
+Lemma subs_tmapp : forall sigma s1 s2,
+  subs sigma (tmapp s1 s2) = tmapp (subs sigma s1) (subs sigma s2).
+Proof.
+  intros sigma s1 s2.
+  induction sigma as [| [x t] sigma' IHsigma'].
+  - reflexivity.
+  - simpl. rewrite IHsigma'. reflexivity.
+Qed.
+
+Lemma subs_tmlam : forall sigma x A s,
+  subs sigma (tmlam x A s) = tmlam x A (subs sigma s).
+Proof.
+  intros sigma x A s.
+  induction sigma as [| [y t] sigma' IHsigma'].
+  - reflexivity.
+  - simpl. rewrite IHsigma'. reflexivity.
+Qed.
+
+Hint Rewrite
+  (* Rewrite rule for application *)
+  subs_tmapp : subs_db.
+
+Hint Rewrite
+  (* Rewrite rule for lambda abstraction *)
+  subs_tmlam : subs_db.
+
+(* Add the lemmas to the hint database *)
+Hint Resolve subs_tmapp : subs_db.
+Hint Resolve subs_tmlam : subs_db.
+
+(* So sub is also rewritten when rewriting subs *)
+Hint Extern 1 => simpl sub : subs_db.
+
+(* todo, current implementation is not correct, there is 
+  no relation between binders in s and t. *)
+Fixpoint to_unique_binders (s : term) := 
+  match s with
+  | tmvar x => tmvar x
+  | tmlam x A s => tmlam x A (to_unique_binders s)
+  | tmapp s t => tmapp (to_unique_binders s) (to_unique_binders t)
+  end.
 
 Lemma to_unique_binders_alpha s : Alpha [] s (to_unique_binders s).
 Admitted.
@@ -66,9 +122,15 @@ Admitted.
 (* If a term has globally unique binders, then it has unique binders*)
 
 Inductive step_gu_naive : term -> term -> Set :=
-| step_gu_naive_intro s t : 
-    step_naive (to_unique_binders s) t ->
+| step_gu_naive_intro s s' t : 
+    Alpha [] s s' ->
+    GU_vars s' ->
+    step_naive s' t ->
     step_gu_naive s t.
+(*     
+    Alpha [] t' t ->
+    GU_vars t ->
+    step_gu_naive s t. *)
 
 (* used to be prop (TODO: Defined also in SN_STCL_named )*)
 Inductive sn {e : term -> term -> Set } x : Set :=
@@ -76,17 +138,1007 @@ Inductive sn {e : term -> term -> Set } x : Set :=
 
 Notation SN_na := (@sn step_gu_naive).
 
+Lemma step_gu_naive_preserves_alpha {s} {s'} {t} ren :
+  Alpha ren s t -> step_gu_naive s s' -> {t' & prod (step_gu_naive t t') (Alpha ren s' t')}.
+Proof.
+Admitted.
+
+Theorem α_preserves_SN_R s s' R :
+  Alpha R s s' -> SN_na s -> SN_na s'.
+Proof.
+  intros Hα Hsn.
+  generalize dependent s'.
+  generalize dependent R.
+  induction Hsn. intros R s' Hα.
+  apply SNI.
+  intros y1 Hstep.
+  assert ({y1_α & prod (step_gu_naive x y1_α) (R ⊢ y1 ~ y1_α)}) as [y1_α [Hstep' Hα'] ].
+  {
+    (* eapply step_gu_naive_preserves_alpha; auto.
+    - eapply alpha_sym in Hα. exact Hα. apply alpha_sym_nil.
+    - assumption. *)
+    admit.
+  }
+  eapply H.
+  - exact Hstep'.
+  - eapply alpha_sym. apply alpha_sym_nil. exact Hα'.
+Admitted.
+
+(* TODO: Can probably be simplified.
+  Both s and s' are alpha equiv to the same GU s_GU. From this they step to the same thing
+*)
+Theorem α_preserves_SN s s' :
+  Alpha [] s s' -> SN_na s -> SN_na s'.
+Proof.
+  intros Hα Hsn.
+  generalize dependent s'.
+  induction Hsn. intros s' Hα.
+  apply SNI.
+  intros y1 Hstep.
+  assert ({y1_α & prod (step_gu_naive x y1_α) (nil ⊢ y1 ~ y1_α)}) as [y1_α [Hstep' Hα'] ].
+  {
+    eapply step_gu_naive_preserves_alpha; auto.
+    - eapply alpha_sym in Hα. exact Hα. apply alpha_sym_nil.
+    - assumption.
+  }
+  eapply H.
+  - exact Hstep'.
+  - eapply alpha_sym. apply alpha_sym_nil. exact Hα'.
+Qed.
+
+Lemma sn_preimage {e : term -> term -> Set} (h : term -> term) x :
+  (forall x y, e x y -> e (h x) (h y)) -> @sn e (h x) -> @sn e x.
+Proof.
+  intros A B.
+  remember (h x) as v. (* this allows us to keep B : sn v as an hypothesis*)
+  generalize dependent h.
+  generalize dependent x.
+  induction B.
+  intros x0 h A eqn.
+  apply SNI.
+  intros y C.
+  apply A in C.
+  specialize (H (h y)).
+  (* apply A in C. *)
+  (* intros C. *)
+  (* apply A in C. *)
+  (* revert C. *)
+  rewrite <- eqn in C.
+  eapply H.
+  - assumption.
+  - exact A.
+  - reflexivity.
+Qed.
+
+(* TODO: It is currently for step only, not for general relation e anymore.
+Idea: Previous lemma sn_preimage above strengthened IH with remember (h x) as v.
+We strenghen IH with (h x) ~ v.
+ *)
+Lemma sn_preimage_α' (h : term -> term) x v :
+  (forall x y, step_gu_naive x y -> {y_h & prod (step_gu_naive (h x) y_h) (nil ⊢ y_h ~ (h y))}) -> @sn step_gu_naive v -> nil ⊢ v ~ h x -> @sn step_gu_naive x.
+Proof.
+  intros A B Halpha.
+  generalize dependent h.
+  generalize dependent x.
+  (* remember (h x) as v. (* this allows us to keep B : sn v as an hypothesis*)
+  generalize dependent h.
+  generalize dependent x.
+  assert (forall x h, (forall x0 y, e x0 y -> {y_h & prod(e (h x0) y_h) (nil ⊢ y_h ~ h y)}) -> nil ⊢ v ~ h x -> @sn e x).
+  {
+  intros x h A. *)
+  (* So we are now not proving sn (h x) -> sn x anymore.
+    We are proving: sn v ->  v ~ h x  -> sn x
+  *)
+  induction B.
+  intros x0 h A eqn.
+  apply SNI.
+  intros y C.
+  apply A in C.
+  (* x ~ h x0.
+    step (h x0) y_h  /\ y_h ~ h y
+
+    exists y_h' s.t. step x y_h' /\ y_h' ~ y_h   ( and then y_h'  ~  h y)
+  *)
+  assert ({y_h' & prod (step x y_h') (nil ⊢ y_h' ~ h y)}).
+  {
+    destruct C as [yh [ehy yh_alpha] ].
+    eapply alpha_sym in eqn; [|apply alpha_sym_nil].
+    apply (step_preserves_alpha nil eqn) in ehy.
+    destruct ehy as [t' [stept' alphat'] ].
+    exists t'.
+    split.
+    - assumption.
+    - eapply alpha_trans.
+      + apply alpha_trans_nil.
+      + eapply alpha_sym. apply alpha_sym_nil. exact alphat'.
+      + assumption.
+  }
+  destruct H0 as [yh' [ehy' yh_alpha'] ].
+  specialize (H yh').
+  eapply H.
+  - assumption.
+  - exact A.
+  - assumption.
+Admitted.
+
+Lemma sn_preimage_α (h : term -> term) x :
+  (forall x y, step_gu_naive x y -> {y_h & prod (step_gu_naive (h x) y_h) (nil ⊢ y_h ~ (h y))}) -> @sn step_gu_naive (h x) -> @sn step_gu_naive x.
+Proof.
+  intros A B.
+  apply sn_preimage_α' with (v := h x) (h := h); eauto.
+  apply alpha_refl. apply alpha_refl_nil.
+Qed.
+
+Lemma sn_closedL t s : SN_na (tmapp s t) -> SN_na s.
+Proof. apply: (sn_preimage (h := tmapp^~t)) => x y.
+(* Maybe this must be up to alpha*)
+Admitted.
+
+Require Import Coq.Program.Equality.
+
+Inductive step_gu_naive_helper : term -> term -> term -> term -> Set :=
+  sgunahIntro s s' t' t :
+    Alpha [] s s' ->
+    GU_vars s' ->
+    step_naive s' t' ->
+    Alpha [] t' t ->
+    GU_vars t ->
+    step_gu_naive_helper s s' t' t.
+
+
+(* Not sure how to call this yet.
+if we have no_capture t sigma
+We want to have unique binders elementwise in sigma.
+No binder in t can occur as free or bound variable in sigma,
+  thus substituting sigma in t will not cause unwanted capture.
+*)
+Inductive no_capture : term -> list (string * term) -> Set :=
+| no_capture_nil t :
+    no_capture t []
+| no_capture_cons t x s sigma :
+    no_capture t sigma ->
+    (forall y, In y (btv t) -> ((y <> x) * (~ In y (tv s)))) -> (* no capturing *)
+    GU_vars s -> (* unique binders in sigma elementwise *)
+    (* 
+      Added to fix soundness
+    Now since multiple institutions should be interpreted as first doing the substs on the right
+      and then the one on the left, we also do not want capture after first doing those on the right
+      
+      Hence, no free var in s nor x itself may be captured by binders in map snd sigma
+      *)
+    (forall y, In y (List.concat (map btv (map snd sigma))) -> ((y <> x) * (~ In y (tv s)))) ->
+    no_capture t ((x, s) :: sigma).
+
+Lemma no_capture_lam x A s sigma :
+  no_capture (tmlam x A s) sigma -> no_capture s sigma.
+Admitted.
+
+Lemma no_capture_app_l s t sigma :
+  no_capture (tmapp s t) sigma -> no_capture s sigma.
+Admitted.
+
+Lemma no_capture_app_r s t sigma :
+  no_capture (tmapp s t) sigma -> no_capture t sigma.
+Admitted.
+
+Lemma assume_first_arg a b :
+  (a -> b) -> b.
+Proof.
+Admitted.
+
+Inductive SubCA : string -> term -> term -> term -> list (string * string) -> Set :=
+| SubCA_intro x U T T' R :
+    Alpha R T T' ->
+    Alpha R U U ->
+    Alpha R (tmvar x) (tmvar x) ->
+    no_capture T' [(x, U)] -> (* x not a binder in T' and no binder in T' is a free var in U*)
+    SubCA x U T (sub x U T') R.
+
+(*
+Sub x U T T1 iff  ⊢ T1 ~ substituteTCA x U T
+*)
+
+(* This would be another way of doing it, where the fourth argument is the term that the
+  subsitution goes to taking into account capture*)
+Lemma commute_sub_16 X σ Tx Tσ s A B C D R:
+  SubCA X Tx s    A R ->
+  SubCA σ Tσ A    B R -> (* this does nto make sense, we would need different R, sicne the rightalpha of this one is used as the left alpha somewhere else*)
+
+  SubCA σ Tσ s    C R ->
+  SubCA σ Tσ Tx   D R ->
+  SubCA X D C     B R.
+
+
+Lemma commute_sub_15 X σ Tx Tσ s :
+  Alpha [] 
+    (sub X (sub σ Tσ Tx) (sub σ Tσ s))
+    (sub σ Tσ (sub X Tx s)).
+
+(* I want to be in a position where the binders are chosen thus that I can do substitueT
+  without checking if we are tyring to substitute a binder:
+    i.e. no checks in substituteT 
+    Then we ahve the property:
+    subsT x t (tmlam y T s) = tmlam y T (subsT x t s) even if x = y (because that cannot happen anymore)
+      Then also no_capture can go into the lambda
+    this can be put into the no_capture property?
+    *)
+  (* Maybe we can leave out the R by switching to a renaming approach? *)
+Lemma commute_sub_naive R x s t (sigma sigma' : list (string * term)) xtsAlpha:
+  Alpha R (sub x t s) xtsAlpha ->
+  αCtxSub R sigma sigma' -> (* TODO: Vars in R not in sigma?*)
+
+  (* these two just say: x not in key or ftv sigma*)
+  ~ In x (map fst sigma) ->
+  (forall ftvs, In ftvs (map snd sigma) -> ~ In x (ftv ftvs)) -> 
+  no_capture xtsAlpha sigma' ->
+  no_capture s [(x, t)] ->
+  no_capture s sigma ->
+  no_capture (subs sigma s) [(x, subs sigma t)] ->
+  (* s.t. substituteTs sigma xtsAlpha does not capture 
+    e.g. suppose sigma:= [y := x]
+    and xtsAlpha = λx. y.
+    then substituting would capture.
+    But we can always choose an alpha equivalent xtsAlpha with 
+    different binder names not occuring in the rhs of sigma
+  *)
+  R ⊢ (sub x (subs sigma t) (subs sigma s))
+      ~ (subs sigma' xtsAlpha).
+
+    (* sub x (subs sigma t) (subs sigma s) ~ subs sigma (sub x t s)
+    
+    Barendreght variable convention source says:
+    - x may not occur as key in sigma.
+    - 
+    *)
+Proof.
+  intros.
+  generalize dependent xtsAlpha.
+  generalize dependent R.
+  induction s; intros.
+  - (* We need to have that x does not occur in lhs or rhs of sigma! We have control over x
+    when calling this function, so we should be good.*)
+    destr_eqb_eq x s.
+    + simpl in H. rewrite String.eqb_refl in H.
+      destruct (in_dec String.string_dec s (map fst sigma)).
+      * (* We know x= s not in keys or values of sigma. hence x=s cannot be in map fst sigma *)
+        admit.
+      * assert (subs sigma (tmvar s) = tmvar s) by admit.
+        rewrite H7.
+        simpl.
+        rewrite String.eqb_refl.
+        (* subs preserves alpha? *)
+        admit.
+    + simpl in H. 
+      rewrite <- String.eqb_neq in H7.
+      rewrite H7 in H.
+      inversion H; subst.
+      destruct (in_dec String.string_dec s (map fst sigma)).
+      * assert ({T & (In (s, T) sigma) * (subs sigma (tmvar s) = T)}%type) by admit.
+        destruct H8 as [T [Hin Hsubs] ].
+        rewrite Hsubs.
+        (* T is in rhs sigma, hence x cannot be in T *)
+        assert (sub x (subs sigma t) T = T) by admit.
+        rewrite H8.
+        (* alpha preserves blablabla (possibly we can enforce that x, y not in R. ? Should not be necessary, but it can be true if that makes it easier)*)
+        admit.
+      * assert (subs sigma (tmvar s) = tmvar s) by admit.
+        rewrite H8.
+        simpl.
+        rewrite H7.
+        (* s not in sigma, then y not in sigma' by alpha *)
+
+
+
+    (* we lookup s in sigma.
+      Case (s, T) in sigma:
+        Goal: sub x (subs sigma t) T ~ subs sigma xtsAlpha
+        We know:    subs sigma (tmvar s) = T.
+      
+      Case s not in sigma:
+        Goal: sub x (subs sigma t) (tmvar s) ~ subs sigma xtsAlpha
+    *)
+    admit.
+  - 
+    (* simpl in H. *)
+    inversion H; subst.
+    autorewrite with subs_db in *.
+    (* simpl sub. *)
+    constructor.
+    eapply IHs; try eapply no_capture_lam; eauto.
+    admit.
+  - simpl in H.
+    inversion H; subst.
+    autorewrite with subs_db in *.
+    constructor. fold sub.
+    + eapply IHs1; eauto; eapply no_capture_app_l; eauto.
+    + eapply IHs2; eauto; eapply no_capture_app_r; eauto.
+Admitted.
+
+(* SEE ALPHA_SUB.v for proof for substituteT, that is prolly easily ported *)
+Lemma substituteT_preserves_alpha_test R U U' T T' X X':
+  (forall Y, In Y (btv T) -> ~ In Y (ftv U)) -> (* this is why we can do substituteT without worrying about capture*)
+  (* We could prevent this maybe by just renaming to globally unique in every lemma*)
+  Alpha R U U' ->
+  Alpha R T T' ->
+  AlphaVar R X X' ->
+  Alpha R (sub X U T) (sub X' U' T').
+Proof.
+Admitted.
+
+(* TODO: MORE CONDITIONS: no shadowing/capture *)
+Lemma subs_preserves_alpha R sigma T T' :
+  false -> (* adding this so we don't forget this is a prototype*)
+  Alpha R T T' ->
+  Alpha R (subs sigma T) (subs sigma T').
+Proof.
+Admitted.
+
+(* Problem: this is not true.
+  after step_gu_naie, t does not have to be globally unique and hence the substitution will capture
+  simplest solution: assume that step_gu_naive does globally uniquing before and after (and implement that later).
+
+  We should have a GU property on sigma, but since sigma is never changed,
+  this will not complicate the induction hypothesis or anything, it
+  will just restrict the applicability of the lemma, which is fine.
+*)
+Lemma step_subst_sigma sigma {s s' t t' } :
+  Alpha [] s s' -> 
+  step_naive s' t -> 
+  GU_vars s' ->
+  no_capture s' sigma -> (* no free vars in sigma are binders in s'*)
+  Alpha [] t t' -> 
+  GU_vars t' ->
+  no_capture t' sigma ->
+  {aT : term & 
+  (step_gu_naive (subs sigma s') aT) * (Alpha [] aT (subs sigma t'))}%type.
+Proof.
+  intros. rename H0 into Hstep. generalize dependent s. generalize dependent t'. induction Hstep; intros.
+  - (* The difficult case. The whole reason we need to do global uniqueness every step
+    *)
+    inversion H; subst. inversion H9; subst.
+    autorewrite with subs_db. 
+    assert ({
+      subSigS & {
+        subSigT & 
+          Alpha [] subSigS (subs sigma s) *
+          Alpha [] subSigT (subs sigma t) *
+          GU_vars (tmapp (tmlam x A (subSigS)) subSigT)
+        }
+      }%type
+    ) by admit.
+    destruct H0 as [subSigS [subSigT [HsubSigS ] ] ].
+    destruct HsubSigS as [HsubSigSAlpha HsubSigTAlpha].
+
+    exists (sub x subSigT subSigS).
+    split.
+    + admit.
+    + 
+    eapply @alpha_trans with (t := sub x (subs sigma t) (subs sigma s)); try constructor.
+    eapply substituteT_preserves_alpha_test.
+    { (* by gu I think *) admit.  } eauto. eauto. constructor.
+    eapply commute_sub_naive; eauto.
+    * admit.
+    * admit.
+    * (* when do we have capture? 
+      If substituting sigma into t' would cause capture
+      This can only happen if t' has binder y e.g.
+      and then sigma contains a y.
+      But that cannot happen by no_binders t' sigma
+      *)
+      admit.
+    * (* by GU_Vars *)
+      admit.
+    * (* by no_binders tmapp (tmlam x A s) t) sigma*)
+      admit.
+     (* That seems more difficult.
+        t has no binders in s or sigma
+        sigma has no binders in t or s
+        free_vars (subs sigma t) <= free_vars t + free_vars sigma
+        we only have capture if there is a binder in subs sigma s that is
+        in those free_vars.
+        binders (subs sigma s) <= binders s + binders sigma
+
+        if y is a binder in s, then it is not free in t by GU_vars
+        if y is a binder in s, then it is not in the free_vars of sigma. by no_binders
+
+        if y is a binder in sigma, then it is not in free_vars sigma (by no shadowing somewhere?)
+        if y is a binder in sigma, then it is not in t by no_binders I think
+      *)
+      
+    
+     
+
+
+
+
+    (* I think we can make assumptions about GU on sigma or something. Then 
+      we rewrite to
+
+
+      tmapp (tmlam x A (subsTs2 sig s)) (subsTs2 sig t0)
+      ALPHA
+      tmapp (tmlam x A subAlphaS      ) (subAlphat0)
+      ->
+      subT x subAlphat0 subAlphaS
+      ALPHA
+      subT x (subsTs2 sig t0) (subsTs2 sig s)    ~   aT
+
+      Magic: x and sig do not interfere: sig has no x in keys or values, 
+      and also sig and (subsTs2 sig t0) do not interfere
+
+      hence:
+
+      subT x t0 (subsTs2 sig s)  ~  subsTs2 sig (subT x t0 s)
+      ALPHA
+      subTs2 sig t.
+
+      We could choose (tmapp (tmlam x A s) t0) in such a way s.t. no binder occurs in sigma
+      However, if sigma contains say a "y".
+      And t0 contains a free "y". Then we cannot change that t0 to not have the free "y"
+    
+    *)
+    
+  
+   (* Assume s and t are globally unique 
+    Induction on step_gu_naive.
+    Four cases:
+    - step_beta: s = tmapp (tmlam x A s1) s2 ->  t_ = subsT x s2 s1, then t = gu t
+    *)
+    * admit.
+    - inversion H; subst.
+
+      assert (GU_vars s1) by admit.
+      specialize (IHHstep H0).
+      apply assume_first_arg in IHHstep.
+      inversion H3; subst.
+      specialize (IHHstep s4 H11).
+      apply assume_first_arg in IHHstep.
+      apply assume_first_arg in IHHstep.
+      specialize (IHHstep s0 H9).
+      destruct IHHstep as [sigS1 [HstepS1 HalphaS1] ]. 
+      autorewrite with subs_db.
+      assert ({sigS1alpha : term & {sigtalpha : term & 
+        (Alpha [] sigS1 sigS1alpha) * 
+        (Alpha [] (subs sigma t) sigtalpha) *
+        GU_vars (tmapp sigS1alpha sigtalpha)
+      } }%type).
+      {
+        (* This is not hard to see:
+          We perform "to_global_unique" on tmapp (sigS1 (substituteTs sigma t))
+          This will yield something alpha equiv to it which is GU_Vars and can be decomposed
+        
+        but how to tell coq?*)
+        admit.
+      }
+      destruct H6 as [sigS1alpha [sigtalpha [ HsigS1alpha ] ] ].
+      destruct HsigS1alpha as [HsigS1alpha HsigtAlpha].
+      exists (tmapp sigS1alpha sigtalpha).
+      (*
+        So, is this the case? The alpha one is true by construction.
+        for step_gu_naive, we need some unfolding lemmas. The only thing it does is first making stuff
+        unique, but keeping alpha equivalence.
+
+        We know that
+
+        substituteTs2 sigma s0 -> sigS1 ~ substituteTs2 sigma s2 ~ sigS1alpha
+
+      Ok. I assume that the other 2 cases are analogous.
+      *)
+      admit.
+    - admit.
+    - inversion H; subst.
+      inversion H3; subst.
+      apply assume_first_arg in IHHstep.
+      apply assume_first_arg in IHHstep.
+      specialize (IHHstep s4).
+      apply assume_first_arg in IHHstep.
+      apply assume_first_arg in IHHstep.
+      apply assume_first_arg in IHHstep.
+      specialize (IHHstep s0).
+      apply assume_first_arg in IHHstep.
+      autorewrite with subs_db.
+      destruct IHHstep as [subSigmaS1_ [Hsteps1 Halpha] ].
+      (* we know no x in sigma and no binders x in s1*)
+      assert ({subSigmaS1 & 
+        Alpha [] subSigmaS1 (subs sigma s1) * 
+        GU_vars (tmlam x A subSigmaS1)
+      }%type).
+      {
+        admit.
+      }
+
+
+  
+Admitted.
+
+Lemma sn_subst X T s : SN_na (sub X T s) -> SN_na s.
+Proof.
+  apply: (sn_preimage_α (h := sub X T)) => x y. exact: step_subst_single.
+Admitted.
+
+Definition cand := term -> Set.
+
+Definition neutral (s : term) : bool :=
+  match s with
+    | tmlam _ _ _ => false
+    | _ => true
+  end.
+
+Record reducible (P : cand) : Set := {
+  p_sn : forall s, P s -> SN_na s;
+  p_cl : forall s t, P s -> step_gu_naive s t -> P t;
+  p_nc : forall s, neutral s -> (forall t, step_gu_naive s t -> P t) -> P s
+}.
+
+(* Since we are only interested in globally unique alpha terms, we do an exists here.
+But we should do a little study if that is necessary.
+
+we want this to hold for [x := t] meaning substituteT:
+Lemma beta_expansion A B x s t :p
+  SN_na t -> L A ([x := t] s) ->
+  L A (tmapp (tmlam x B s) t).
+
+It also has to hold for A := Kind_Base, in which case it is proved by showing SN_na.
+We only have that these two terms mean the same thing if we are allowed to forget about capture in the sbustitution
+Hence only if t is globally unique with respect to s. We can enforce that by changing the definition of L.
+
+JACCO and WOUTER think it is a bad idea to change the LR and that using L_preserves_alpha will allow us to use original LR.
+
+*)
+Fixpoint L (T : type) : cand :=
+match T with
+  | tp_base => SN_na 
+  | tp_arrow A B => fun s => forall t, L A t -> L B (tmapp s t)
+end.
+
+
+
+Fixpoint L2 (T : type) : cand :=
+match T with
+  | tp_base => SN_na 
+  (* this is a restriction on the t that we want to accept.
+  However, these types of programs that we no longer allow are not GU_Vars, something like
+  
+  (λx.λy. x) y
+  This would not be allowed, but we can always find an alpha equivalent s for which this particular t would be allowed.
+  *)
+  | tp_arrow A B => fun s => forall t, L2 A t -> GU_vars (tmapp s t) -> L2 B (tmapp s t)
+end.
+
+(* integrally depends on α_preserves_SN *)
+Lemma α_preserves_L A s s' :
+  Alpha [] s s' -> L A s -> L A s'.
+Proof.
+  intros.
+  generalize dependent s.
+  generalize dependent s'.
+  induction A; intros.
+  - simpl. simpl in H0.
+    apply α_preserves_SN with s; assumption.
+  - simpl in H0.
+    simpl.
+    intros t Ht.
+    specialize (H0 t Ht).
+    assert (nil ⊢ (tmapp s t) ~ (tmapp s' t)).
+    {
+      apply alpha_app.
+      - assumption.
+      - apply alpha_refl. apply alpha_refl_nil.
+    }
+    specialize (IHA2 (tmapp s' t) (tmapp s t) H1 H0).
+    assumption.
+Qed.
+
+Lemma α_preserves_L_R A s s' R :
+  Alpha R s s' -> L A s -> L A s'.
+Proof.
+  intros.
+  generalize dependent s.
+  generalize dependent s'.
+  generalize dependent R.
+  induction A; intros.
+  - simpl. simpl in H0.
+    eapply α_preserves_SN_R with (s := s); eauto.
+  - simpl in H0.
+    simpl.
+    intros t Ht.
+    assert ({t0 & Alpha R t0 t}) as [t0 Halphat0] by admit.
+    specialize (H0 t0).
+    specialize (IHA1 (sym_alpha_ctx R) t0 t).
+    assert (sym_alpha_ctx R ⊢ t ~ t0) by admit.
+    specialize (IHA1 H1 Ht).
+    assert (R ⊢ (tmapp s t0) ~ (tmapp s' t)).
+    {
+      apply alpha_app; assumption.
+    }
+    
+    specialize (IHA2 R (tmapp s' t) (tmapp s t0) H2 (H0 IHA1)).
+    assumption.
+Admitted.
+
+Lemma reducible_sn : reducible SN_na.
+Proof. 
+  constructor; eauto using ARS.sn. by move=> s t [f] /f. 
+  intros s.  elim: s => //.
+Qed.
+
+Global Hint Resolve reducible_sn : core.
+
+Lemma reducible_var P x : reducible P -> P (tmvar x).
+Proof. move/p_nc. apply=> // t st. 
+(* There is no t s.t. step_gu_naive (tmvar x) t*)
+Admitted.
+
+Lemma L_reducible A :
+  reducible (L A).
+Proof with eauto using step_gu_naive.
+  elim: A => /=[|A ih1 B ih2].
+  - apply reducible_sn.
+  - constructor.
+    + move=> s h. apply: (@sn_closedL (tmvar "x")). apply: (p_sn (P := L B))...
+      eapply h. eapply reducible_var; eauto.
+    + move=> s t h st u la. apply: (p_cl _ (s := tmapp s u))...
+      apply step_gu_naive_intro. inversion st; subst.  apply: step_appL. apply: h. apply: p_sn...
+    + move=> s ns h t la.
+      have snt := p_sn ih1 la.
+      elim: snt la => {} t _ ih3 la. apply: p_nc... move=> v st. inv st=> //...
+      (* Note: Case L B ([x := t] s0. By using Autosubst's "inv" instead of normal inversion, this goal vanishes. Why? *) (* Todo: Think, this case doesn't happen in db variant*)
+      * apply: ih3 => //. exact: (p_cl ih1) la _.
+Admitted.
+
+Corollary L_sn A s : L A s -> SN_na s.
+Proof. intros Las. assert (reducible (L A)) by apply (L_reducible A).
+   apply (p_sn H). assumption.
+Qed.
+
+Corollary L_cl T s t : L T s -> step_gu_naive s t -> L T t.
+Proof.
+  intros Hstep Hst.
+  assert (H: reducible (L T)) by apply L_reducible.
+  apply (p_cl H Hstep); assumption.
+Qed.
+
+Corollary L_nc T s :
+  neutral s -> (forall t, step_gu_naive s t -> L T t) -> L T s.
+Proof. 
+  intros Hneut Hstep.
+  assert (H: reducible (L T)) by apply L_reducible.
+  apply (p_nc H); assumption.
+Qed.
+
+Corollary L_var T x : L T (tmvar x).
+Proof.
+  apply L_nc; first by []. intros t st. inversion st.
+Admitted. 
+
+Inductive star {e : term -> term -> Set } (x : term) : term -> Set :=
+| starR : star x x
+| starSE y z : star x y -> e y z -> star x z.
+
+
+(** **** Many-Step Reduction 
+TODO: See if we can use the star from autosubst ARS again. (uses Prop instead of Set)
+*)
+Definition red_gu_na := @star step_gu_naive.
+
+Corollary L_cl_star T s t :
+  L T s -> red_gu_na s t -> L T t.
+Proof.
+  intros Ls red_st. induction red_st.
+  - assumption.
+  - apply L_cl with y; assumption.
+Qed.
+
 (* If we have substituteT X U s, we need some assumption that U and s already have unique bindrs*)
 
-Lemma step_gu_naive_subst s t U X : 
-  step_gu_naive s t -> 
-  {α : term & 
-  (step_gu_naive (substituteT X U s) α) * (nil ⊢ α ~ (substituteT X U t))} .
-Proof.
-    intros.
-    inversion H; subst.
-    (* ok... we need some guarantees that free vars are not changed by to_unique_binders*)
+Definition EL (Gamma : list (string * type)) 
+          (sigma : list (string * term)) : Set :=
+  forall x T, lookup x Gamma = Some T ->
+    { t & prod (lookup x sigma = Some t) (L T t)}.
 
+(* is true! *)
+Lemma extend_EL (Gamma : list (string * type)) (sigma : list (string * term)) x T t :
+  EL Gamma sigma -> L T t -> EL ((x, T) :: Gamma) ((x, t) :: sigma).
+Proof.
+Admitted.
+
+Reserved Notation "Δ '|-*' T ':' K" (at level 40, T at level 0, K at level 0).
+Inductive has_type : list (string * type) -> term -> type -> Set :=
+  | K_Var : forall Δ X K,
+      List.lookup X Δ = Some K ->
+      Δ |-* (tmvar X) : K
+  | K_Lam : forall Δ X K1 T K2,
+      ((X, K1) :: Δ) |-* T : K2 ->
+      Δ |-* (tmlam X K1 T) : (tp_arrow K1 K2)
+  | K_App : forall Δ T1 T2 K1 K2,
+      Δ |-* T1 : (tp_arrow K1 K2) ->
+      Δ |-* T2 : K1 ->
+      Δ |-* (tmapp T1 T2) : K2
+where "Δ '|-*' T ':' K" := (has_type Δ T K).
+
+
+Lemma red_beta_gu_na x s t1 t2 :
+  step_gu_naive t1 t2 ->
+  { α & prod 
+      (red_gu_na (substituteT x t1 s) α)
+      (nil ⊢ α ~ (substituteT x t2 s))
+  }.
+Proof.
+  intros Hstep.
+  eapply red_beta'; auto; 
+    solve [try apply alpha_refl; try apply alphavar_refl; constructor].
+Admitted.
+
+(* Closure under beta expansion. *)
+Lemma beta_expansion A B x s s' t :
+  Alpha [] s' s ->
+  no_capture s' [(x, t)] -> (* this really is the right assumption. no free variable in t is a binder in s', because these binders could be added to the environment through beta reduction and then capture*)
+  SN_na t -> L A (sub x t s') -> (* Key: s' is GU now *)
+  L A (tmapp (tmlam x B s) t).
+Proof with eauto.
+  move=> alphass' guvars snt h. have sns := sn_subst (L_sn h).
+  assert (SN_na s).
+  {
+    eapply α_preserves_SN; eauto.
+  } 
+  clear sns.
+  generalize dependent h.
+  generalize dependent s'.
+  induction H. intros.
+  (* generalize dependent s.
+
+  (* TODO: How to get that second IH? *)
+
+  induction sns. intros. *)
+  apply: L_nc => // u st. 
+  (* assert ({u' & Alpha [] u u' * step_naive (tmapp (tmlam x B s) t) u'}%type) as st' by admit.
+  destruct st' as [u' [au' st'] ]. *)
+  assert (step_naive (tmapp (tmlam x B s') t) u) as st' by admit.
+    
+  inv st' => //.
+  (* - apply α_preserves_L with (s := sub x t s); auto. eapply alpha_sym. econstructor. auto. *)
+  - inv H3.
+    assert (Hprr: step_gu_naive x0 s0) by admit.
+    specialize (H s0 Hprr).
+    assert({s'0_nc & Alpha [] s'0_nc s0 * no_capture s'0_nc [(x, t)]}%type) by admit.
+    destruct H0 as [s'0_nc [Hreds0_nc Hno_caps0] ].
+    specialize (H s'0_nc Hreds0_nc Hno_caps0).
+
+    (* inversion au'; subst. inversion H3; subst.  *)
+    (* assert (step_gu_naive s s0) by admit. assumes no_capture also says something about uniqueness in term *)
+    apply H => //.
+    (* s steps naively to s0. Could make it non-unique, but it could not have caused new binders like x and t*)
+    (* assert ({s0' & Alpha [] s0 s0' * no_capture s0' [(x, t)]}%type) as [s0' [Hreds0' Hno_caps0'] ].
+    {
+      admit.
+    } *)
+
+    assert ({α & (step_gu_naive (sub x t s') α) * (nil ⊢ α ~ sub x t s'0_nc)}%type) 
+      as [alpha [Hred Halpha] ].
+      {
+        eapply (@step_subst_sigma ((x, t)::nil)).
+        - apply alpha_refl. constructor.
+        - eauto. 
+        - admit.
+        - assumption.
+        - eapply alpha_sym; eauto. constructor.
+        - admit.
+        - eauto.
+      }
+    
+     
+    
+    apply (L_cl h) in Hred.
+    apply α_preserves_L with (s := alpha); assumption.
+  - (* presumably analogous to above? *)
+Admitted.
+
+
+Lemma beta_expansion_subst X t sigma s A B :
+  no_capture (subs sigma s) [(X, t)] ->
+  SN_na t -> L A (subs ((X, t)::sigma) s) -> L A (tmapp (subs sigma (tmlam X B s)) t).
+Proof.
+(* to remove the no_capture assumption
+  we generate s' s.t. no_capture (subs sigma s) [(X, t)].
+  not possible, what if the binder is in rhs of sigma.
+  well, it should also be allowed to change the rhs's of sigma to alpha equivalent terms.
+*)
+  intros nc snt H.
+  simpl in H.
+  eapply beta_expansion in H.
+  - autorewrite with subs_db. eauto.
+  - apply alpha_refl. constructor.
+  - assumption.
+    (* again we need an alpha step here that transforms subs sigma s to something GU in some sense
+    *) 
+  - assumption. 
+Qed.
+
+Lemma no_capture_helper s X t sigma :
+  no_capture s ((X, t)::sigma) -> no_capture (subs sigma s) [(X, t)].
+Admitted.
+
+(* I devised this to make soundness var case easier, but is not getting easier
+  so maybe I try to switch to paralell substs anyway.
+*)
+Inductive Blabla : list (string * term) -> Set :=
+| Blabla_nil : Blabla []
+| Blabla_cons x t sigma :
+    Blabla sigma -> 
+    ~ In x (List.concat (map ftv (map snd sigma))) -> 
+    Blabla ((x, t)::sigma).
+(* This says that one subsitutions does not have effect on the next one
+  In other word, no substiutions chains, where x -> t, and then t -> y, etc.
+
+  This also means that if we define lookup as right oriented, that
+    lookup_left x sigma = Some T   -> subs sigma (tmvar x) = T
+*)
+
+(* The fundamental theorem. *)
+Theorem soundness_ex Gamma s sigma' s' A R:
+  has_type Gamma s A -> 
+  forall sigma,
+    EL Gamma sigma -> 
+    (* Blabla sigma -> (* this will say that we cannot have sigmas like [x |-> y] ([z |-> x] s) *)
+      in other words, the next subsitution has no effect if the previous one suceeded.
+    *)
+    (* Blabla sigma -> *)
+    Blabla sigma' -> (* this still allows identity substitutions, we could put this into EL*)
+    Alpha R s s' -> 
+    αCtxSub R sigma sigma' -> (* TODO: Once this works, why do we even need this? sigma and sigma' are all free to choose, why do we not just choose original sigma to not be captured??? *)
+    (* no_capture s sigma -> *)
+    no_capture s' sigma' -> (* shouldnt be too strong. we only want to use this for identity substitutions. And even by design only substituting free variables (so no free var in sigma should be a bound var in s)*)
+    (L A (subs sigma' s')).
+Proof.
+  intros.
+  generalize dependent R.
+  generalize dependent s'.
+  generalize dependent sigma.
+  generalize dependent sigma'.
+  induction H.
+  - intros.
+    inversion H2; subst. clear H4.
+    eapply α_preserves_L with (s := subs sigma (tmvar X)).
+    (* Everything in sigma is L by EL Δ sigma*)
+    (* Then by alpha also for sigma' and then also X in sigma' and value alpha equivalent to the one in sigma*)
+    (* So also L
+        The above can be summarised as: sub_preserves_alpha
+    *)
+
+    (* What if it is not in sigma'? variables are automatically L*)
+    + admit.
+    + unfold EL in H0.
+      specialize (H0 X K e).
+      destruct H0 as [t [HlookupSigma LAt] ].
+      (* problem. what if first X is subsituted for Y, and then that is again substituted
+        This is because we no longer have parallel substitutions.
+
+        ok. but. suppose it is like (subs sigma1 (subs sigma2 X)) and then in subs sigma2 X, it indeed
+        subsitutes for t which is L.
+        
+      *)  
+    admit.
+  - 
+    intros.
+    simpl.
+    intros.
+    inversion H2; subst.
+    (* this says: we can rename binders in rhs of sigma' and s' so that no capturign occurs *)
+    assert ({s'' & { sigma'' &  Alpha [] s2 s'' *
+      (* no_capture (tmlam X K1 s'') sigma''  * TODO: Oof. We cannot enforce this, because now we say: X not in sigma'' *)
+      no_capture s'' ((y, t)::sigma'') * 
+      αCtxSub [] sigma' sigma'' *
+      no_capture (subs sigma'' s'') [(y, t)]
+      }}%type) by admit.
+
+    assert ({t0 & Alpha ((X, y)::R) t0 t}) as [t0 Halphat0] by admit.
+
+    destruct H6 as [s'' [sigma'' [ [ [ Halpha Hno_cap ] Hctx ] Hnocapsubs ] ] ].
+    
+    specialize (IHhas_type ((y, t)::sigma'')).
+      assert (Hblabla: Blabla ((y, t)::sigma'')).
+      {
+        constructor; auto.
+        (* alpha preserves blabla (yes, because alpha doesnt change freevars )*)
+        admit.
+        (* by no_capture (tmlam y K1 s2) sigma'
+            y is a binder in the term.
+            So that means that y is not free in any of the values of sigma', 
+              and also not in the keys of sigma'
+
+              by aphaCtxSub [] sigma' sigma'' we have that they have the same ftvs, so it also holds for sigma''
+        *)
+        admit.
+      }
+      specialize (IHhas_type Hblabla ((X, t0)::sigma)).
+      apply assume_first_arg in IHhas_type.
+
+
+      
+
+      specialize (IHhas_type s'' Hno_cap ((X, y)::R)).
+      apply assume_first_arg in IHhas_type.
+      assert (αCtxSub ((X, y)::R) ((X, t0)::sigma) ((y, t)::sigma'')) by admit.
+      (* This notion assumes a different definition of αCtxSub
+        Every substitution corresponds to a beta reduction.
+        We already had the subsitutions with R sigma and sigma''
+        let's make that less abstract
+        [x -> t]   and   [y -> t']    and R = [x, y] ??
+        origingating from 
+        (λz. (λx. s) t) U    and  (λz'. (λy. s') t') U'
+      *)
+      specialize (IHhas_type H6).
+      
+      
+      eapply beta_expansion_subst in IHhas_type.
+      + eapply α_preserves_L; [|exact IHhas_type].
+        constructor; [|eapply alpha_refl; constructor].
+        apply subs_preseserves_alpha.
+        admit.
+
+
+      + auto.
+      + apply L_sn in H5. auto.
+  - intros.
+    inversion H3; subst.
+    autorewrite with subs_db.
+    specialize (IHhas_type2 sigma' H1 sigma).
+    specialize (IHhas_type1 sigma' H1 sigma).
+    apply assume_first_arg in IHhas_type1.
+    apply assume_first_arg in IHhas_type2.
+    specialize (IHhas_type1 s2).
+    specialize (IHhas_type2 t2).
+    apply assume_first_arg in IHhas_type1.
+    apply assume_first_arg in IHhas_type2.
+    specialize (IHhas_type1 R H9 H5).
+    specialize (IHhas_type2 R H11 H5).
+    eauto.
+Admitted.
+
+(* The fundamental theorem. *)
+Theorem soundness Gamma s A :
+  has_type Gamma s A -> forall sigma,
+    EL Gamma sigma -> L A (subs sigma s).
+Proof with eauto using L_sn. 
+  elim=> {Gamma s A} [Gamma X A |Gamma X A s B _ ih sigma EL|Gamma s t A B _ ih1 _ ih2 sigma HEL].
+  - intros HlookupGamma sigma HEL.
+    unfold EL in HEL.
+    specialize (HEL X A HlookupGamma).
+    destruct HEL as [t [HlookupSigma LAt] ].
+    admit.
+  - move=> t h.
+    specialize (ih ((X, t)::sigma) (extend_EL EL h)).
+
+    (* The key everytime is that we can move to an alpha equivalent term that is nice to work with
+        i.e. does not have shadowing and is globally unqiue, and can have some properties like
+          unique wrt sigma *)
+    assert({s' & Alpha [] s s' * no_capture s' ((X, t)::sigma)}%type) by admit.
+    destruct H as [s' [Halphas Hno_caps'] ].
+    assert (Alpha [] (subs ((X, t) :: sigma) s) (subs ((X, t)::sigma) s')).
+    {
+      eapply subs_preserves_alpha.
+      - admit.
+      - assumption.
+    }
+    assert (L B (subs ((X, t) :: sigma) s')).
+    {
+      eapply α_preserves_L in ih; eauto.
+    }
+    eapply beta_expansion_subst in H0; eauto.
+    + eapply α_preserves_L with (s := tmapp (subs sigma (tmlam X A s')) t); eauto.
+      constructor.
+      * autorewrite with subs_db.
+        constructor.
+        admit.
+      * apply alpha_refl. constructor.
+    +  admit.
+    + apply L_sn in h. assumption.
+  - autorewrite with subs_db.
+    specialize (ih1 _ HEL).
+    specialize (ih2 _ HEL).
+    unfold L in ih1. fold L in ih1.
+    specialize (ih1 (subs sigma t) ih2).
+    assumption.
 Admitted.
 
 
